format-version: 1.2
date: 02:09:2010 17:01
saved-by: Thorsten Henrich
default-namespace: platynereis_stage

[Typedef]
id: OBO_REL:begins_at_end_of
name: begins at end of

[Term]
id: PD_ST:0000090
name: Platynereis developmental stage
namespace: platynereis_stage
def: "A Platynereis developmental stage is an occurrent that is a temporal subdivision of a Platynereis dumerilii development." [PLATY:T_Henrich]
comment: Developmental stages are typically demarcated by the timing of appearance, loss or transformation of specific anatomical structures.

[Term]
id: PD_ST:0000100
name: Zygote stage
synonym: "0-2 zyg" [PLATY:A.H.L.Fischer]
namespace: platynereis_stage
def: "First developmental stage with the following key events: Fertilized egg before the onset of cleavage. Jelly forms, cortical migration of lipid droplets." [PLATY:A.H.L.Fischer]
is_a: PD_ST:0000090
comment: At a temperature of 18 C this stages lasts from 0.00 hours till 2.00 hours.

[Term]
id: PD_ST:0000200
name: Cleaving embryo stage
synonym: "2-7 cle" [PLATY:A.H.L.Fischer]
namespace: platynereis_stage
def: "Developmental stage following Zygote stage with the following key events: Spiral cleavage pattern with individually identifiable blastomeres. First and second cleavage inequal and meridional. Third cleavage forms micromeres and macromeres. Ends with the appearance of the fourth quartette of micromeres." [PLATY:A.H.L.Fischer]
is_a: PD_ST:0000090
comment: At a temperature of 18 C this stages lasts from 2.00 hours till 7.00 hours.
relationship: OBO_REL:begins_at_end_of PD_ST:0000100

[Term]
id: PD_ST:0000300
name: Stereoblastula - Stereogastrula stage
synonym: "7-13 ste" [PLATY:A.H.L.Fischer]
namespace: platynereis_stage
def: "Developmental stage following Cleaving embryo stage with the following key events: Spherical mass of dividing blastomeres whose cell lineage can no longer be followed by eye. Micromeres divide bilaterally. Epibody starts." [PLATY:A.H.L.Fischer]
is_a: PD_ST:0000090
comment: At a temperature of 18 C this stages lasts from 7.00 hours till 13.00 hours.
relationship: OBO_REL:begins_at_end_of PD_ST:0000200

[Term]
id: PD_ST:0000400
name: Protrochophore stage
synonym: "13-24 pt" [PLATY:A.H.L.Fischer]
namespace: platynereis_stage
def: "Developmental stage following Stereoblastula - Stereogastrula stage with the following key events: Pre-larva, slowly rotating in the jelly driven by the multi-ciliated equatorial prototroch cells. Apical tuft appears." [PLATY:A.H.L.Fischer]
is_a: PD_ST:0000090
comment: At a temperature of 18 C this stages lasts from 13.00 hours till 24.00 hours.
relationship: OBO_REL:begins_at_end_of PD_ST:0000300

[Term]
id: PD_ST:0000500
name: Early trochophore stage
synonym: "24-26 et" [PLATY:A.H.L.Fischer]
namespace: platynereis_stage
def: "Developmental stage following Protrochophore stage with the following key events: Hatching larvae actively swimming in the water column, but yet without phototaxis. First pigment appears in the larval eyes. Telotroch forms apical ganglion forms. One serotonergic cell in the brain. First larval brain axon. Prototroch nerve develops. Ventral nerve cord is v-shaped." [PLATY:A.H.L.Fischer]
is_a: PD_ST:0000090
comment: At a temperature of 18 C this stages lasts from 24.00 hours till 26.00 hours.
relationship: OBO_REL:begins_at_end_of PD_ST:0000400

[Term]
id: PD_ST:0000600
name: Mid-trochophore stage
synonym: "26-40 mt" [PLATY:A.H.L.Fischer]
namespace: platynereis_stage
def: "Developmental stage following Early trochophore stage with the following key events: Free-swimming trochophores showing phototaxis. Increasing amount of shading pigment in the larval eyes. Stomodeal rosette starts forming and moves anteriorly. The body shape starts to change from spherical to conical. Variable: red pigment spots around the prototroch cells. Second cerebral commissure, future nuchal organ nerve and asymmetric axon develop. Three more serotonergic cells around apical ganglion. First commissure in the ventral nerve cord. Dorsal and ventral longitudinal muscles appear." [PLATY:A.H.L.Fischer]
is_a: PD_ST:0000090
comment: At a temperature of 18 C this stages lasts from 26.00 hours till 40.00 hours.
relationship: OBO_REL:begins_at_end_of PD_ST:0000500

[Term]
id: PD_ST:0000700
name: Late trochophore stage
synonym: "40-48 lt" [PLATY:A.H.L.Fischer]
namespace: platynereis_stage
def: "Developmental stage following Mid-trochophore stage with the following key events: Distinct stomodeal opening surrounded by stomodeal rosette, first chaetae visible within the trunk. Three larval segments appear simultaneously, identifiable by the developing chaetae in the trunk. Macromeres narrower towards the posterior. Second commissure forms in the ventral nerve cord. Dorsal and ventral longitudinal muscles elongate." [PLATY:A.H.L.Fischer]
is_a: PD_ST:0000090
comment: At a temperature of 18 C this stages lasts from 40.00 hours till 48.00 hours.
relationship: OBO_REL:begins_at_end_of PD_ST:0000600

[Term]
id: PD_ST:0000800
name: Early metatrochophore stage
synonym: "48-51 emt" [PLATY:A.H.L.Fischer]
namespace: platynereis_stage
def: "Developmental stage following Late trochophore stage with the following key events: Formation of the first paratroch at the posterior border of the second chaetigerous segment, chaetae reach the body wall. Number of cells contributing to the stomodeal rosette is slowly increasing. Red pigment at the telotroch can appear. Third commissure forms in the ventral nerve cord. Second and third pair of serotonergic cells in the ventral nerve cord. Oblique and parapodial muscles more numerous and elongate." [PLATY:A.H.L.Fischer]
is_a: PD_ST:0000090
comment: At a temperature of 18 C this stages lasts from 48.00 hours till 51.00 hours.
relationship: OBO_REL:begins_at_end_of PD_ST:0000700

[Term]
id: PD_ST:0000900
name: Mid-metatrochophore stage
synonym: "51-60 mmt" [PLATY:A.H.L.Fischer]
namespace: platynereis_stage
def: "Developmental stage following Early metatrochophore stage with the following key events: Pigment of the adult eyes clearly visible lateral-dorsally in the episphere. Chaetae outside the body wall, but parapodia not yet formed. Amount of pigment in the adult eyes increases. Chaetae elongate. The gut anlage becomes visible. Additional ring of cells surrounds the stomodeal opening from anterior to posterior. Stomodeum starts to invaginate into the head. Second paratroch forms at the posterior border of the first chaetigerous trunk segments. Increasing number of axons in the commissures. Convergent extension movements start in the ventral neuroectoderm and continue until 72hpf (Steinmetz et al., 2007). Fourth pair of serotonergic cells in the ventral nerve cord. Ventral medial longitudinal muscle starts forming." [PLATY:A.H.L.Fischer]
is_a: PD_ST:0000090
comment: At a temperature of 18 C this stages lasts from 51.00 hours till 60.00 hours.
relationship: OBO_REL:begins_at_end_of PD_ST:0000800

[Term]
id: PD_ST:0001000
name: Late metatrochophore stage
synonym: "60-66 lmt" [PLATY:A.H.L.Fischer]
namespace: platynereis_stage
def: "Developmental stage following Mid-metatrochophore stage with the following key events: Parapodia visible but cannot move yet. Chaetae of the third chaetigerous segment reach to the posterior end of the larvae.
Body shape changes from conical to torpedo-like and slender. Formation of the akrotroch starts. Stomodeal opening becomes slit-like. Ventral medial longitudinal muscle elongates." [PLATY:A.H.L.Fischer]
is_a: PD_ST:0000090
comment: At a temperature of 18 C this stages lasts from 60.00 hours till 66.00 hours.
relationship: OBO_REL:begins_at_end_of PD_ST:0000900

[Term]
id: PD_ST:0001100
name: Early nectochaete stage
synonym: "66-75 en" [PLATY:A.H.L.Fischer]
namespace: platynereis_stage
def: "Developmental stage following Late metatrochophore stage with the following key events: Parapodia start moving independently. Formation of the metatroch. Akrotroch fully developed. Rapid elongation of the trunk. Antennae not visible yet. Anlage of the proctodeum becomes visible. Occasionally larvae crawl using their parapodia. Much stronger pigmentation in the adult eyes. Lipid droplets move posteriorly. 1-2 pigmented spots at the basis of each parapodium. Dorsal and ventral roots of the circumesophageal connectives approach each other. Further serotonergic cells in the ventral nerve cord. Muscles form anteriorly to the stomodeum." [PLATY:A.H.L.Fischer]
is_a: PD_ST:0000090
comment: At a temperature of 18 C this stages lasts from 66.00 hours till 75.00 hours.
relationship: OBO_REL:begins_at_end_of PD_ST:0001000

[Term]
id: PD_ST:0001200
name: Mid-nectochaete stage
synonym: "75-6d mn" [PLATY:A.H.L.Fischer]
namespace: platynereis_stage
def: "Developmental stage following Early nectochaete stage with the following key events: Formation of the antero-dorsal pair of tentacular cirri, anal cirri and antennal stubs. Body shape changes from torpedo-like into worm-like. Head distinguishable from the trunk due to a constriction. Adult eyes grow in size and are only separated by a medial constriction. Jaws start forming. Macromeres start to cellularize and begin to form midgut epithelium. Proctodeum develops a cylindrical tube shape. The stomodeum and proctodeum get in contact with the midgut (Hauenschild and Fischer, 1969). Pigmented spots at the base of the parapodia increase in size. Additional pigment appears in the head region. Brain grows. Additional serotonergic cells in the brain. Segmental nerves can be identified. Muscles and nerves of the antennae, tentacular cirri anal cirri become visible." [PLATY:A.H.L.Fischer]
is_a: PD_ST:0000090
comment: At a temperature of 18 C this stages lasts from 75.00 hours till 96.00 hours.
relationship: OBO_REL:begins_at_end_of PD_ST:0001100

[Term]
id: PD_ST:0001300
name: Late nectochaete stage
synonym: "6d-2w ln" [PLATY:A.H.L.Fischer]
namespace: platynereis_stage
def: "Developmental stage following Mid-nectochaete stage with the following key events: Antennae elongate, palpi become visible, beginning of food intake. The antennae become long and slender. Palpi form on both sides of the mouth opening. The gut becomes functional and the larvae begin to feed. The midgut lumen is only slit-like. Lipid droplets begin to be resorbed to variable degree. Jaws grow rapidly and a secondary tooth is added. Transition progresses from pelago-benthic to fully benthic lifestyle. Brain continues to grow rapidly. Two additional serotonergic cells in the brain. Musculature around the stomodeum increases in complexity and a basket of muscles develops around the jaws to form the pharynx. Muscles and nerves, which are associated with the developing antennae, tentacular cirri, palpi and anal cirri increase in length. End of synchronized development." [PLATY:A.H.L.Fischer]
is_a: PD_ST:0000090
comment: At a temperature of 18 C this stages lasts from 96.00 hours till 168.00 hours.
relationship: OBO_REL:begins_at_end_of PD_ST:0001200

[Term]
id: PD_ST:0001410
name: Three-segmented errant juvenile stage
synonym: "3 seg" [PLATY:A.H.L.Fischer]
namespace: platynereis_stage
def: "Developmental stage following Late nectochaete stage with the following key events: No lipid droplets visible in the gut barrel-shaped midgut filled with food. Settlement metamorphosis completed during this stage. Growth of the fourth chaetigerous segment. Lipid droplets are totally resorbed. Jaws rapidly increase in size. More teeth are added. Spinning glands develop and start to form mucus. Palpi elongate slowly. Antennae, antero-dorsal tentacular cirri and anal cirri elongate rapidly. By the end of this stage, the forth chaetigerous segment is fully formed." [PLATY:A.H.L.Fischer]
is_a: PD_ST:0000090
relationship: OBO_REL:begins_at_end_of PD_ST:0001300

[Term]
id: PD_ST:0001510
name: 4- and 5-segmented errant juvenile stage
synonym: "4-5 seg" [PLATY:A.H.L.Fischer]
namespace: platynereis_stage
def: "Developmental stage following Three-segmented errant juvenile stage with the following key events: Fourth chaetigerous body segment fully formed; fifth chaetigerous segment growing or fully formed. Jaws grow rapidly and more teeth are added. The antero-ventral tentacular cirri form. Fifth chaetigerous segment is formed by the posterior growth zone. Pharynx develops into an eversible proboscis." [PLATY:A.H.L.Fischer]
is_a: PD_ST:0000090
relationship: OBO_REL:begins_at_end_of PD_ST:0001410

[Term]
id: PD_ST:0001520
name: Cephalic metamorphosis stage
synonym: "ceph m" [PLATY:A.H.L.Fischer]
namespace: platynereis_stage
def: "Developmental stage following 4- and 5-segmented errant juvenile stage with the following key events: Loss of chaetae at the first pair of parapodia, which marks the beginning of the transformation of the first pair of parapodia into the posterior pair of tentacular cirri. The juveniles undergo cephalic metamorphosis by transforming the first pair of parapodia into the posterior pair of tentacular cirri. Larval eyes seem to disappear during metamorphosis. Palpi and antennae elongate slowly. Midgut elongates rapidly with the elongating body. Jaws grow in size and more teeth are added. Larvae build characteristic tubes in which they live." [PLATY:A.H.L.Fischer]
is_a: PD_ST:0000090
relationship: OBO_REL:begins_at_end_of PD_ST:0001510

[Term]
id: PD_ST:0001530
name: Small atokous worm stage
synonym: "s atok" [PLATY:A.H.L.Fischer]
namespace: platynereis_stage
def: "Developmental stage following Cephalic metamorphosis stage with the following key events: Cephalic metamorphosis is finished and the posterior pairs of tentacular cirri are formed. The posterior growth zone buds off a series of further segments. Less than fifty segments. Anterior segments grow in size. The diameter of the worm increases." [PLATY:A.H.L.Fischer]
is_a: PD_ST:0000090
relationship: OBO_REL:begins_at_end_of PD_ST:0001520

[Term]
id: PD_ST:0001540
name: Large atokous worm stage
synonym: "l atok" [PLATY:A.H.L.Fischer]
namespace: platynereis_stage
def: "Developmental stage following Small atokous worm stage with the following key events: Tubicolous worm with more than 50 segments. Sexually immature atokous worms start to produce gametes in the coelom. Growth rate slows until they possess up to 70 segments and the gametes start to mature within the body cavity." [PLATY:A.H.L.Fischer]
is_a: PD_ST:0000090
relationship: OBO_REL:begins_at_end_of PD_ST:0001530

[Term]
id: PD_ST:0001550
name: Sexual metamorphosis stage
synonym: "sex" [PLATY:A.H.L.Fischer]
namespace: platynereis_stage
def: "Developmental stage following Large atokous worm stage with the following key events: End of food intake resulting in an empty gut. Eyes increase in size. Some of the chromatophores degenerate. Maturing females are yellow and maturing males are whitish (anterior) and red (posterior). Posterior parapodia flatten and develop paddle-like chaetae. Major portion of the musculature degenerate and new a muscle type for rapid swimming develops." [PLATY:A.H.L.Fischer]
is_a: PD_ST:0000090
relationship: OBO_REL:begins_at_end_of PD_ST:0001540

[Term]
id: PD_ST:0001600
name: Adult (Heteronereis) stage
synonym: "adult" [PLATY:A.H.L.Fischer]
namespace: platynereis_stage
def: "Developmental stage following Sexual metamorphosis stage with the following key events: Rapid swimming in straight lines. Nuptial dance. Synchronized by lunar periodicity. Mature animals become pelagic. Swarming and nuptial dance. The females release the eggs through disruptions/ fissures between the segments. Males release the sperm through a number of newly formed papillae at the posterior end. The eggs are fertilized in the water. After spawning, males and females die." [PLATY:A.H.L.Fischer]
is_a: PD_ST:0000090
relationship: OBO_REL:begins_at_end_of PD_ST:0001550
